module BTA3 where

open import Data.Nat
open import Data.Bool
open import Data.List

-- Binding times
data BT : Set where
  S : BT
  D : BT

-- defining a data type [BT],where two members are
-- [S] standing for "static" and [D] standing for dynamic.

-- ``subsumption'' binding times; static can be treated as dynamic,
-- but not vice versa
_≼_ : BT → BT → Bool
_≼_ D S  = false
_≼_ _ _  = true

-- note that the above function can also be specified as follows,
-- _≼_ : BT → BT → Bool 
-- D ≼ S = false
-- _ ≼ _ = true

-- note that the function [≼] specifies that a "static",S, can be treated
-- as a "dynamic",D, and not the other way round
-- since in Agda, pattern matching is conducted in a sequencial fashion,
-- the above specification makes sure that it returns [false] when the 
-- first argument is [D] and the second [S] and returns [true] in all
-- the other three cases.




-- BEGIN: stuff that is also in the standard library

-- Standard propositional equality, see also Relation.Binary.PropositionalEquality
data _==_ {A : Set} (x : A) : A → Set where
  refl : x == x
-- [_==_] defines an equality proposition
-- it takes two identical elements of one type as arguments and gives one 
-- evidence,[refl],for the proposition

-- subst lemma
subst : {A B : Set}{x x' : A} {C : A → B} → x == x' → C x == C x'
subst{A}{B}{x}{.x} refl = refl

-- or being defined in the following manner...
-- my_subst : {A B : Set}{x x' : A}{C : A → B} →  x == x' → C x == C x'
-- my_subst refl = refl

-- the above function further helps to construct evidence for equality 
-- proposition
-- it says that if two elements are identical then two new elements obtained
-- by applying the former to a function  should also be identical



record True : Set where
data False : Set where

-- note that the above is regarding two simple proposition [True] and [False]
-- regarding [True],
-- it is defined as empty record with a single element of type [True],[record{}]
-- the trick here is that the type checker knows this and fills in any implicit
-- arguments of [True] with this element
-- another way of defining [True] as follows,
-- record True : Set where
-- trivial : True
-- trivial = _

-- regarding [False],
-- it is defined as a proposition without any evidence corresponding well to
-- what a [False] proposition really means

isTrue : Bool → Set
isTrue true  = True
isTrue false = False
-- note the isTrue b,given b as boolean, is the type of proof that b is equal to
-- true since if it is the case, [isTrue b] returns type [True] where its
-- evidence is automatically filled in by the type checker while if it is not
-- the case there is no way to supply for the evidence due to the way how 
-- [false] is constructed 


-- END standard library

----------------------
-- Sublists
----------------------
data _cx-≤_ {A : Set} : List A → List A → Set where
  cxle-eq : (l : List A) → l cx-≤ l
  cxle-lt : ∀ {l₁ l₂} x → l₁ cx-≤ l₂ → l₁ cx-≤ (x ∷ l₂)


lem-cx-≤-trans : {A : Set} → {l₁ : List A} {l₂ : List A} {l₃ : List A} →
                 l₁ cx-≤ l₂ → l₂ cx-≤ l₃ → l₁ cx-≤ l₃
lem-cx-≤-trans le1  (cxle-eq l) = le1
lem-cx-≤-trans (cxle-eq l) (cxle-lt x e) = cxle-lt x e
lem-cx-≤-trans (cxle-lt x e) (cxle-lt x' e') = cxle-lt x' (lem-cx-≤-trans (cxle-lt x e) e')
 


_cxle-∷_ : {A : Set} (x : A) (l : List A) → l cx-≤ (x ∷ l)
x cxle-∷ l = cxle-lt x (cxle-eq l)


data _⊆_ {A : Set} : List A → List A → Set where
  refl-⊆ : ∀ {l} → l ⊆ l
  step-⊆ : ∀ {l} x l₁ l₂ → l ⊆ (l₁ ++ l₂) → l ⊆ (l₁ ++ (x ∷ l₂))

lem-⊆-trans : {A : Set} → {l₁ : List A} {l₂ : List A} {l₃ : List A} →
                 l₁ ⊆ l₂ → l₂ ⊆ l₃ → l₁ ⊆ l₃
lem-⊆-trans e (refl-⊆ {l}) = e
lem-⊆-trans (refl-⊆ {l}) (step-⊆ x l₁ l₂ e) = step-⊆ x l₁ l₂ e
lem-⊆-trans (step-⊆ x l₁ l₂ e) (step-⊆ x' l₁' l₂' e') = step-⊆ x' l₁' l₂' (lem-⊆-trans (step-⊆ x l₁ l₂ e) e') 

-- data _≤1_ {A : Set} : List A → List A → Set where
--   cxle1-eq : (l : List A) → l ≤1 l
--   cxle1-lt : ∀ x (l : List A) → l ≤1 (x ∷ l)

 
-- data _?∷_ {A : Set} (x : A): List A → Set where
--   yes∷ : (l : List A) → x ?∷ (x ∷ l)
--   no∷ : (l : List A) → x ?∷ l

-- getList : ∀ {A} {x : A} {l : List A} → x ?∷ l → List A
-- getList {x = x} (yes∷ l) = x ∷ l
-- getList {_} {_} {l} (no∷ .l) = l

-- end sublists

-- some lemmas about BT subsumption
lem-bt≼S : {bt : BT} → isTrue (bt ≼ S) → bt == S
lem-bt≼S {S} bt≼S = refl
lem-bt≼S {D} ()

-- which can also be defined as follows,
-- my_lem-bt≼S : {bt : BT} → isTrue (bt ≼ S) → bt == S
-- my_lem-bt≼S {S} _ = refl
-- my_lem-bt≼S {D} ()

lem-D≼bt : {bt : BT} → isTrue (D ≼ bt) → bt == D
lem-D≼bt {S} ()
lem-D≼bt {D} D≼bt = refl


-- Types of the calculus
mutual
  -- s ^ BT
  data AType : Set where
    Ann : BT → SType → AType

  -- int | t -> t
  data SType : Set where
    SInt  : SType
    SFun  : AType → AType → SType


-- aux definitions
ATInt : BT → AType
ATInt bt = Ann bt SInt
ATFun  : BT → AType → AType → AType
ATFun  bt at1 at2 = Ann bt (SFun at1 at2)

-- note that the above function labels a ground type with annotations [S] or
-- [D],sort of a labelling function

-- projection: get the BT from a type
btof : AType → BT
btof (Ann bt _) = bt

-- a related function which takes an annotated type as argument and returns
-- the annotation of that type

-- "constraint on types: functions have to be at least as dynamic as their component" should be corrected as follows,
-- arguments of function should be as dynamic as the function

data wft : AType → Set where
  wf-int  : ∀ {bt} → wft (Ann bt SInt)
  wf-fun  : ∀ {bt at1 at2} → wft at1 → wft at2
          → isTrue (bt ≼ btof at1) → isTrue (bt ≼ btof at2) → wft (Ann bt (SFun at1 at2))

-- the above proposition specifies a set of well-formed [AType]s,
-- any annotated [SInt]s are well-formed, wft (Ann bt SInt) forall bt ∈ BT
-- in case of functional type with annotation, the following two criteria have
-- to be satisfied to be a well form,
-- a. each of its arguments is well-formed
-- b. the annotation of the function and the annotations of its arguments must
--    satisfy [_≼_] relation
--    for instance, the functional type defined above is well-formed while
--    the following is not,
--    Ann D (
--            SFun (Ann S SInt) (Ann D SInt)
--          )
--    in conclusion,for functional type with annotation to be well-formed,
--    each of its arguments annotations has to be [D] when that of the function
--    is [D] while there is no constraint upon the annotations of its arguments
--    when that of the function is [S]

lem-force-bt : ∀ {bt at} → isTrue (bt ≼ btof at) → D == bt → D == btof at
lem-force-bt {S} bt≼at ()
lem-force-bt {D} {Ann S y'} () D=bt
lem-force-bt {D} {Ann D y'} bt≼at D=bt = refl

-- note the above function takes an element[bt] of type [BT] and a type with 
-- annotation,
-- if both 
-- a. the type is at least as dynamic as [bt]
-- b. [bt == D]
-- then we know that the annotation of the type must be [D] as well
-- and the function in that case returns evidence for that

-- Low-level types; types wihtout binding information
data Type : Set where
  TInt : Type
  TFun : Type → Type → Type

-- translation from ATypes to low-level types
mutual
  strip : AType → Type
  strip (Ann _ σ) = strip' σ

  strip' : SType → Type
  strip' SInt = TInt
  strip' (SFun y y') = TFun (strip y) (strip y')

-- note that the above function [strip] converts a type with annotation [AType]
-- to a low-level type [Type],
-- for instance,
-- strip (Ann D SInt)
-- = strip' SInt
-- = TInt
-- strip (Ann S
--         SFun (Ann S SInt) (Ann D SInt)
--       )
-- = strip' (SFun (Ann S SInt) (Ann D SInt))
-- = TFun (strip (Ann S SInt)) (strip (Ann D SInt))
-- = TFun (strip' SInt) (strip' SInt) 
-- = TFun TInt TInt^

-- More general purpose definitions (should also be in standard library)
-- list membership
infix 4 _∈_
data _∈_ {A : Set} : A → List A → Set where
  hd : ∀ {x xs} → x ∈ (x ∷ xs)
  tl : ∀ {x y xs} → x ∈ xs → x ∈ (y ∷ xs)

-- note the above proposition gives us two constructors for getting
-- evidences for an element being a member of one list 

-- end general purpose definitions 

-- Typing context
Ctx = List Type

--data Exp' (Γ Γ' : Ctx) : Type → Set where
--  EVar' : 

-- Typed expression
data Exp (Γ : Ctx) : Type → Set where
  -- [EVar] corresponds to the bounded variables in [AExp]
  EVar : ∀ {τ} → τ ∈ Γ → Exp Γ τ
  EInt : ℕ → Exp Γ TInt
  EFun : ∀ {τ₁ τ₂} → Exp (τ₂ ∷ Γ) τ₁ → Exp Γ (TFun τ₂ τ₁)
  EApp : ∀ {τ₁ τ₂} → Exp Γ (TFun τ₂ τ₁) → Exp Γ τ₂ → Exp Γ τ₁
-- one additional term,
count_tl : ∀ {τ Γ Γ'} → τ ∈ Γ → Γ cx-≤ Γ' → τ ∈ Γ'
count_tl  x (cxle-eq Γ) = x
count_tl x  (cxle-lt T e) = tl (count_tl x e)


data _cx=≤_ {A : Set} : List A → List A → Set where
  cxle-peq : ∀ {l₁ l₂} { x } → l₁ cx-≤ l₂ → (x ∷ l₁) cx=≤ (x ∷ l₂)
  cxle-plt : ∀ {l₁ l₂} { x } → l₁ cx=≤ l₂ → (x ∷ l₁) cx=≤ (x ∷ l₂)

get_cx-≤ : ∀{Γ₁ Γ₂ Γ₃ Γ₄} → Γ₁ cx=≤ Γ₂ → Γ₃ cx-≤ Γ₄ 
get_cx-≤ (cxle-plt e) = get_cx-≤ e
get_cx-≤ (cxle-peq e) = e

_id≤Bid_ : ∀{τ Γ Γ'} → τ ∈ Γ → Γ cx=≤ Γ' → Bool
(tl x) id≤Bid (cxle-plt e) = x id≤Bid e
hd id≤Bid e = true
(tl x) id≤Bid (cxle-peq e) = false

lem-x-weakening : ∀{τ Γ Γ'} → (x : τ ∈ Γ) → (e : Γ cx=≤ Γ') → isTrue (x id≤Bid e) → τ ∈ Γ'
lem-x-weakening = {!!}


lem-Exp-weakening' : ∀ {τ₂ τ₁ Γ Γ'} → Exp (τ₂ ∷ Γ) τ₁ → (τ₂ ∷ Γ) cx=≤ (τ₂ ∷ Γ') → Exp (τ₂ ∷ Γ') τ₁
lem-Exp-weakening' (EVar x) e with x id≤Bid e
lem-Exp-weakening'  (EVar x) e | true = EVar (lem-x-weakening x e _ )
lem-Exp-weakening'  (EVar x) e | false = EVar (count_tl x (get_cx-≤ e))
lem-Exp-weakening'  (EInt n) e = EInt n
lem-Exp-weakening'  (EFun t) e = EFun (lem-Exp-weakening' t (cxle-plt e))
lem-Exp-weakening'  (EApp t1 t2) e = EApp (lem-Exp-weakening' t1 e) (lem-Exp-weakening' t2 e)   

lem-Exp-weakening : ∀ {τ Γ Γ'} → Exp Γ τ → Γ cx-≤ Γ' → Exp Γ' τ
lem-Exp-weakening t (cxle-eq Γ) = t
lem-Exp-weakening (EInt n) e = EInt n
lem-Exp-weakening (EVar x) e  = EVar (count_tl x e)
lem-Exp-weakening (EFun t) (cxle-lt T e) = EFun (lem-Exp-weakening' t (cxle-peq (cxle-lt T e))) 
lem-Exp-weakening (EApp t1 t2) e = EApp (lem-Exp-weakening t1 e) (lem-Exp-weakening t2 e)


-- typed annotated expressions
ACtx = List AType

data AExp (Δ : ACtx) : AType → Set where
  AVar : ∀ {α} → α ∈ Δ → AExp Δ α
  AInt : (bt : BT) → ℕ → AExp Δ (ATInt bt)
  AFun : ∀ {α₁ α₂} (bt : BT) → wft (ATFun bt α₂ α₁) → AExp (α₂ ∷ Δ) α₁ → AExp Δ (ATFun bt α₂ α₁)
  AApp : ∀ {α₁ α₂} (bt : BT) → wft (ATFun bt α₂ α₁) → AExp Δ (ATFun bt α₂ α₁) → AExp Δ α₂ → AExp Δ α₁


-- stripping of contexts
residual : ACtx → Ctx
residual [] = []
residual (Ann S _ ∷ xs) = residual xs
residual (Ann D σ ∷ xs) = strip' σ ∷ residual xs

-- ``semantic domain'' for partially evaluated AExp-terms:
--   - AExp-terms of dynamic type evaluate to Exp-terms
--   - AExp-terms of static type evaluate to agda terms, where SFun
--     are functions and SInt are natural numbers
mutual 
  impTA : Ctx → AType → Set
  impTA Γ (Ann S σ) = impTA' Γ σ
  impTA Γ (Ann D σ) = Exp Γ (strip' σ)
  
  impTA' : Ctx → SType → Set
  impTA' Γ SInt = ℕ
  -- impTA' Γ (SFun y y') = impTA Γ y → impTA Γ y'
  impTA' Γ (SFun y y') = ∀ {Γ'} → Γ cx-≤ Γ' → impTA Γ' y → impTA Γ' y'

lem-impTA-weakening : ∀ {α Γ Γ'} →
                      impTA Γ α →
                      Γ cx-≤ Γ' →
                      impTA Γ' α
lem-impTA-weakening {Ann S SInt} v _ = v
lem-impTA-weakening {Ann S (SFun x x₁)} f prf = λ prf' → f (lem-cx-≤-trans prf prf')
lem-impTA-weakening {Ann D x₁} v prf = lem-Exp-weakening v prf 

-- mutual 
--   impTA-try : Ctx → AType → Set
--   impTA-try Γ (Ann S σ) = impTA-try' Γ σ
--   impTA-try Γ (Ann D σ) = Exp Γ (strip' σ)
  
--   impTA-try' : Ctx → SType → Set
--   impTA-try' Γ SInt = ℕ
--   impTA-try' Γ (SFun y y') = impTA-try Γ y → impTA-try Γ y'

-- lem-impTA-try-weakening : ∀ {α Γ Γ'} →
--                       impTA-try Γ α →
--                       Γ cx-≤ Γ' →
--                       impTA-try Γ' α
-- lem-impTA-try-weakening {Ann S SInt} v _ = v
-- lem-impTA-try-weakening {Ann S (SFun α x₁)} {Γ} {Γ'} f prf = {! λ (v : impTA-try Γ' α) → f v!}
-- lem-impTA-try-weakening {Ann D x₁} v prf = lem-Exp-weakening v prf 

data AEnv : Ctx → ACtx → Set where
  env[] :  ∀ {Γ} → AEnv Γ []
  envS:: : ∀ {Γ Δ} {α} →
           impTA Γ α → 
           AEnv Γ Δ →
           AEnv Γ (α ∷ Δ)
  envD:: : ∀ {Γ Δ} →
           (σ : SType) →
           impTA (strip' σ ∷ Γ) (Ann D σ) →
           AEnv Γ Δ →
           AEnv (strip' σ ∷ Γ) (Ann D σ ∷ Δ)


lem-AEnv-weakening : ∀ {Γ Γ' Δ} → AEnv Γ Δ → Γ cx-≤ Γ' → AEnv Γ' Δ
lem-AEnv-weakening env[] prf = env[]
lem-AEnv-weakening (envS:: {α = α} x env) prf = envS:: (lem-impTA-weakening {α} x prf) (lem-AEnv-weakening env prf)
lem-AEnv-weakening (envD:: {Γ} σ x env) prf = envS:: (lem-impTA-weakening {Ann D σ} x prf) (lem-AEnv-weakening env (lem-cx-≤-trans (cxle-lt (strip' σ) (cxle-eq Γ)) prf))  -- non-primitive recursion... this should be fixable by extending Γ in the middle, rather than in the end

lookup : ∀ {Γ Δ α} → AEnv Γ Δ → (o : α ∈ Δ ) → impTA Γ α
lookup env[] ()
lookup (envS:: x env) hd = x
lookup (envS:: x env) (tl idx) = lookup env idx
lookup (envD:: σ x env) hd = x 
lookup {α = α} (envD:: {Γ} σ x env) (tl idx) = lem-impTA-weakening {α} (lookup env idx) (strip' σ cxle-∷ Γ) 

data IsDynamic : AType → Set where
  is-dyn : ∀ σ → IsDynamic (Ann D σ)

lem-IsDynamic-by-wf : ∀ α → isTrue (D ≼ btof α) → IsDynamic α
lem-IsDynamic-by-wf (Ann S σ) ()
lem-IsDynamic-by-wf (Ann D σ) _ = is-dyn σ 

-- TODO: Do we need additional assurance in the type signature (or as
-- an aux. lemma) that Γ is the residue of Δ?
pe : ∀ {Δ Γ α} → AEnv Γ Δ → AExp Δ α → impTA Γ α
pe env (AVar idx) = lookup env idx
pe env (AInt S i) = i
pe env (AInt D i) = EInt i
pe {Γ = Γ} env (AFun {α₁} {α₂} S prf exp) = λ {Γ'} (prf₁ : Γ cx-≤ Γ') (v : impTA Γ' α₂) →
                                                     pe (envS:: v (lem-AEnv-weakening env prf₁)) exp
pe env (AFun {α₁} {α₂} D (wf-fun _ _ prf-2 prf-1) e)
  with lem-IsDynamic-by-wf α₁ prf-1 | lem-IsDynamic-by-wf α₂ prf-2
pe {Γ = Γ} env (AFun {.(Ann D σ₁)} {.(Ann D σ₂)} D (wf-fun _ _ prf-1 prf-2) e)
  | is-dyn σ₁ | is-dyn σ₂ =
  EFun (pe (envD:: σ₂ (EVar hd) env) e)
pe {Γ = Γ} env (AApp S _ f e) = (pe env f (cxle-eq Γ)) (pe env e)
pe env (AApp {α₁} {α₂} D (wf-fun _ _ prf-2 prf-1) f e)
  with lem-IsDynamic-by-wf α₁ prf-1 | lem-IsDynamic-by-wf α₂ prf-2
pe env (AApp {.(Ann D σ₁)}{.(Ann D σ₂)} D (wf-fun _ _ prf-2 prf-1) f e)
 | is-dyn σ₁ | is-dyn σ₂ =
 EApp (pe env f) (pe env e) -- construct an Exp-application using the proof that argument and results are dynamic and thus pe yields Exp-terms for them


